Martin Escardo & Tom de Jong, June 2023.

This is to be added to the file Iterative.ordinals when it is complete.

\begin{code}

{-# OPTIONS --safe --without-K --exact-split --lossy-unification #-}

open import MLTT.Spartan
open import UF.Univalence

module Iterative.Ordinals-more
        (𝓤 : Universe)
        (ua : Univalence)
       where

open import UF.FunExt
open import UF.UA-FunExt

private
 𝓤⁺ : Universe
 𝓤⁺ = 𝓤 ⁺

 fe : Fun-Ext
 fe = Univalence-gives-Fun-Ext ua

 fe' : FunExt
 fe' 𝓤 𝓥 = fe {𝓤} {𝓥}

open import Iterative.Multisets 𝓤
open import Iterative.Sets 𝓤 ua
open import MLTT.W
open import Ordinals.Equivalence
open import Ordinals.Notions
open import Ordinals.OrdinalOfOrdinals ua
open import Ordinals.Type hiding (Ord)
open import Ordinals.Underlying
open import Ordinals.WellOrderTransport
open import UF.Equiv-FunExt
open import UF.Base
open import UF.Embeddings
open import UF.Equiv
open import UF.EquivalenceExamples
open import UF.PairFun
open import UF.Size
open import UF.Subsingletons
open import UF.Subsingletons-FunExt


open import Iterative.Ordinals 𝓤 ua

𝕆-to-Ord-lemma : (α : 𝕆) (x : 𝕆-root α)
               → (𝕆-to-Ord α) ↓ x ＝ 𝕆-to-Ord (𝕆-forest α x)
𝕆-to-Ord-lemma α x = eqtoidₒ (ua 𝓤) fe (𝕆-to-Ord α ↓ x) (𝕆-to-Ord (𝕆-forest α x)) (f , {!!} , {!!})
 where
  f : ⟨ (𝕆-to-Ord α) ↓ x ⟩ → ⟨ 𝕆-to-Ord (𝕆-forest α x) ⟩
  f (a , l) = pr₁ II
   where
    I : 𝕆-forest α a < 𝕆-forest α x
    I = ⌜ 𝕆-to-Ord-order α a x ⌝⁻¹ l

    II : Σ y ꞉ 𝕆-root (𝕆-forest α x) , 𝕆-forest (𝕆-forest α x) y ＝ 𝕆-forest α a
    II = ⌜ <-behaviour (𝕆-forest α a) (𝕆-forest α x) ⌝ I

  g : ⟨ 𝕆-to-Ord (𝕆-forest α x) ⟩ → ⟨ (𝕆-to-Ord α) ↓ x ⟩
  g y = a , l
   where
    have-y : 𝕆-root (𝕆-forest α x)
    have-y = y
    IV : 𝕆-forest (𝕆-forest α x) y < 𝕆-forest α x
    IV = 𝕆-forest-is-< (𝕆-forest α x) y
    III : Σ a ꞉ 𝕆-root α , 𝕆-forest α a ＝ 𝕆-forest (𝕆-forest α x) y
    III = 𝕆-forest-is-lower-closed α x (𝕆-forest (𝕆-forest α x) y) IV
    a : 𝕆-root α
    a = pr₁ III
    p : 𝕆-forest (𝕆-forest α x) y ＝ 𝕆-forest α a
    p = (pr₂ III)⁻¹
    II : Σ y ꞉ 𝕆-root (𝕆-forest α x) , 𝕆-forest (𝕆-forest α x) y ＝ 𝕆-forest α a
    II = y , p
    I : 𝕆-forest α a < 𝕆-forest α x
    I = ⌜ <-behaviour (𝕆-forest α a) (𝕆-forest α x) ⌝⁻¹ II
    l : a ≺⟨ 𝕆-to-Ord α ⟩ x
    l = ⌜ 𝕆-to-Ord-order α a x ⌝ I

  fg : f ∘ g ∼ id
  fg y = {!!}

𝕆-to-Ord-preserves-< : (α β : 𝕆) → α < β → 𝕆-to-Ord α ⊲ 𝕆-to-Ord β
𝕆-to-Ord-preserves-< α β l = II I
 where
  I : Σ y ꞉ 𝕆-root β , 𝕆-forest β y ＝ α
  I = ⌜ <-behaviour α β ⌝ l

  II : type-of I → 𝕆-to-Ord α ⊲ 𝕆-to-Ord β
  II (y , refl) = IV
   where
    III : 𝕆-to-Ord (𝕆-forest β y) ＝ (𝕆-to-Ord β ↓ y)
    III = (𝕆-to-Ord-lemma β y)⁻¹

    IV : 𝕆-to-Ord (𝕆-forest β y) ⊲ 𝕆-to-Ord β
    IV = y , III

Ord-to-𝕆-is-equiv : is-equiv Ord-to-𝕆
Ord-to-𝕆-is-equiv = embeddings-with-sections-are-equivs
                     Ord-to-𝕆
                     Ord-to-𝕆-is-embedding
                     (𝕆-to-Ord , η)
 where
  f : (α : 𝕆)
    → ((x : 𝕆-root α) → Ord-to-𝕆 (𝕆-to-Ord (𝕆-forest α x)) ＝ 𝕆-forest α x)
    → Ord-to-𝕆 (𝕆-to-Ord α) ＝ α
  f α g =
   Ord-to-𝕆 (𝕆-to-Ord α) ＝⟨ I ⟩
   𝕆-ssup (𝕆-root α) (λ x → Ord-to-𝕆 (𝕆-to-Ord α ↓ x)) a b ＝⟨ II ⟩
   𝕆-ssup (𝕆-root α) (λ x → Ord-to-𝕆 (𝕆-to-Ord (𝕆-forest α x))) {!!} {!!} ＝⟨ {!!} ⟩
   {!!} ＝⟨ III ⟩
   𝕆-ssup (𝕆-root α) (𝕆-forest α) {!!} {!!} ＝⟨ 𝕆-η α ⟩
   α ∎
    where
     a = Ord-to-𝕆↓-is-embedding (𝕆-to-Ord α)
     b = Ord-to-𝕆↓-is-lower-closed (𝕆-to-Ord α)
     I   = Ord-to-𝕆-behaviour (𝕆-to-Ord α)
     II  = ap (λ - → 𝕆-ssup (𝕆-root α) (Ord-to-𝕆 ∘ -) {!!} {!!}) (dfunext fe (𝕆-to-Ord-lemma α))
     III = ap (λ - → 𝕆-ssup (𝕆-root α) - {!!} {!!}) (dfunext fe g)

  η : Ord-to-𝕆 ∘ 𝕆-to-Ord ∼ id
  η = 𝕆-induction' _ f

Ordinals-≃ : Ord ≃ 𝕆
Ordinals-≃ = Ord-to-𝕆 , Ord-to-𝕆-is-equiv

𝕆-to-Ord-reflects-< : (α β : 𝕆) → 𝕆-to-Ord α ⊲ 𝕆-to-Ord β → α < β
𝕆-to-Ord-reflects-< α β (y , p) = III
 where
  I = 𝕆-to-Ord (𝕆-forest β y) ＝⟨ (𝕆-to-Ord-lemma β y)⁻¹ ⟩
      (𝕆-to-Ord β ↓ y)        ＝⟨ p ⁻¹ ⟩
      𝕆-to-Ord α              ∎

  II : 𝕆-forest β y ＝ α
  II = equivs-are-lc ⌜ Ordinals-≃ ⌝⁻¹ ⌜ Ordinals-≃ ⌝⁻¹-is-equiv I

  III : α < β
  III = ⌜ <-behaviour α β ⌝⁻¹ (y , II)


Ordinals-agreementₒ : 𝓞 ≃ₒ OO 𝓤
Ordinals-agreementₒ = ⌜ Ordinals-≃ ⌝⁻¹ ,
                      order-preserving-reflecting-equivs-are-order-equivs
                       𝓞
                       (OO 𝓤)
                       ⌜ Ordinals-≃ ⌝⁻¹
                       ⌜ Ordinals-≃ ⌝⁻¹-is-equiv
                       𝕆-to-Ord-preserves-<
                       𝕆-to-Ord-reflects-<

Ordinals-agreement : 𝓞 ＝ OO 𝓤
Ordinals-agreement = eqtoidₒ (ua 𝓤⁺) fe 𝓞 (OO 𝓤) Ordinals-agreementₒ

\end{code}
